counter theorem unfinished

examples/count/verif.v
@@ -90,6 +90,7 @@ Notation P4String := (P4String.t Info).
 
 Module BitArray.
   Definition t := (list Z).
+  Definition zeros (l : Z):= repeat 0 (Z.to_nat l).
 
   Section Operations.
     Variable (width : positive).
@@ -103,14 +104,71 @@ Module BitArray.
   End Operations.
 End BitArray.
 
-
-Definition NUM_ENTRY := 2.
+Definition NUM_ENTRY : Z := 2.
 Definition WIDTH : positive := 4.
 
-Definition ast_match (st : state) (ast : BitArray.t) : Prop :=
-  exists content,
-  PathMap.get !["main"; "ig"; "myCounter"] (snd st) = Some (ObjRegister (mk_register 4%nat NUM_ENTRY content)) /\
-  content = ast.
+Definition process (fbit : Z) (a : BitArray.t) : (BitArray.t * Z) :=
+  if fbit =? 1 then
+    (BitArray.incr WIDTH a 1, 48)
+  else
+    (BitArray.incr WIDTH a 0, 0).
+
+Definition process_multi (fbits : list Z) : (BitArray.t) :=
+  List.fold_left (fun a fbit => fst (process fbit a)) fbits (BitArray.zeros NUM_ENTRY).
+
+Definition fbit_1_count (fbits: list Z) : Z :=
+  List.fold_left (fun c fbit => BitArith.plus_mod WIDTH c 1) (List.filter (Z.eqb 1) fbits) 0.
+
+Lemma process_multi_index_1'' :
+  forall fbits init init2,
+  Znth 1 (List.fold_left (fun a fbit => fst (process fbit a)) fbits (upd_Znth 0 (upd_Znth 1 (BitArray.zeros NUM_ENTRY) init) init2)) =
+  List.fold_left (fun c fbit => BitArith.plus_mod WIDTH c 1) (List.filter (Z.eqb 1) fbits) init.
+  (* Znth 1 (process_multi fbits) = fbit_1_count fbits. *)
+Proof.
+  intros. induction fbits as [|hd tl H].
+  - reflexivity.
+  - unfold BitArray.zeros.
+    destruct (Z.eqb 1 hd) eqn:Hhd; unfold process_multi, fbit_1_count, fold_left, process, filter; intros;
+    rewrite Hhd; rewrite Z.eqb_sym in Hhd; rewrite Hhd.
+    + unfold BitArray.incr. simpl. Search upd_Znth.
+      assert (forall {A:Type} i j (l : list A) u v, 0 <= i < Zlength l -> 0 <= j < Zlength l ->  i <> j -> upd_Znth i (upd_Znth j l u) v = upd_Znth j (upd_Znth i l v) u).
+Admitted.
+
+Lemma process_multi_index_1' :
+  forall fbits init,
+  Znth 1 (List.fold_left (fun a fbit => fst (process fbit a)) fbits (upd_Znth 1 (BitArray.zeros NUM_ENTRY) init)) =
+  List.fold_left (fun c fbit => BitArith.plus_mod WIDTH c 1) (List.filter (Z.eqb 1) fbits) init.
+  (* Znth 1 (process_multi fbits) = fbit_1_count fbits. *)
+Proof.
+  intros fbits. induction fbits as [|hd tl H].
+  - reflexivity.
+  - unfold BitArray.zeros.
+    destruct (Z.eqb 1 hd) eqn:Hhd; unfold process_multi, fbit_1_count, fold_left, process, filter; intros;
+    rewrite Hhd; rewrite Z.eqb_sym in Hhd; rewrite Hhd.
+    + unfold BitArray.incr. simpl. 
+      assert (0 <= 1 < Zlength [0; 0]). 
+      { split. lia. reflexivity. }
+      apply upd_Znth_same with (u := init) in H0. rewrite H0. apply H.
+    + unfold BitArray.incr. simpl. 
+Admitted.
+
+Lemma process_multi_index_1 :
+  forall fbits,
+    Znth 1 (process_multi fbits) = fbit_1_count fbits.
+Proof.
+Admitted.
+
+Lemma process_multi_index_1_original :
+forall fbits,
+  Znth 1 (process_multi fbits) =
+  BitArith.mod_bound WIDTH (Zlength (List.filter (Z.eqb 1) fbits)).
+Proof.
+Admitted.
+
+  
+
+Definition array_in_state (st : state) (a : BitArray.t) : Prop :=
+  PathMap.get !["main"; "ig"; "myCounter"] (snd st) = Some (ObjRegister (mk_register 4%nat NUM_ENTRY a)).
 
 Definition field_contains (v : Val) (name : P4String) (data: Val) : Prop :=
   match v with
@@ -119,11 +177,6 @@ Definition field_contains (v : Val) (name : P4String) (data: Val) : Prop :=
   | _ => False
   end.
 
-Definition process (width : positive) (fbit : Z) (ast : BitArray.t) : (BitArray.t * Z) :=
-  if fbit =? 1 then
-    (BitArray.incr width ast 1, 48)
-  else
-    (BitArray.incr width ast 0, 0).
 
 Section Experiment1.
 Variable fbit : Z.
@@ -140,7 +193,7 @@ Definition pre (* (fbit : Z) (hdr meta standard_metadata : Val) *) (in_args : li
   /\ field_contains hdr !"firstBit" (ValBaseBit 1%nat fbit)
   /\ (exists counter, field_contains meta !"counter" (ValBaseBit (Z.to_nat (Z.pos WIDTH)) counter))
   /\ (exists eport, field_contains standard_metadata !"egress_spec" (ValBaseBit 9%nat eport))
-  /\ ast_match st ast.
+  /\ array_in_state st ast.
 
 Definition post (* (fbit : Z) (hdr meta standard_metadata : Val) *) (out_args : list Val) (st : state) :=
   let (ast', eport) := process WIDTH fbit ast in
@@ -158,7 +211,7 @@ Definition post (* (fbit : Z) (hdr meta standard_metadata : Val) *) (out_args : 
     /\ Ops.eval_binary_op_eq (ValBaseStruct (AList.filter std_meta_fields (P4String.equivb !"egress_spec" )))
                              (ValBaseStruct (AList.filter std_meta_fields' (P4String.equivb !"egress_spec" )))
        = Some true
-    /\ ast_match st ast'.
+    /\ array_in_state st ast'.
 
 (* Lemma body_counter : hoare_func ge inst_m this pre myFundef nil post.
 Abort. *)
